Framework.v
@@ -15,13 +15,31 @@ Proof.
 Lemma s_body_to_term_abs : forall ts,
   s_body ts -> s_term (s_trm_abs ts).
 Proof.
-  intros. inversion H. Abort.
+  intros. inversion H. pick fresh x0.
+  apply s_term_abs with (L := x).
+  intros. apply H0. apply H1.
+Qed.
 
-Hint Resolve s_term_abs_to_body.
+Hint Resolve s_term_abs_to_body s_body_to_term_abs.
 
 Lemma s_subst_id : forall t x u,
   x \notin s_fv t -> [x ~> u]t = t.
-Proof. Abort.
+Proof.
+  intros.
+  induction t using s_trm_mutind with 
+  (P := fun t => x `notin` s_fv t -> [x ~> u] t = t);
+  intros; simpl.
+    - induction x0. reflexivity. simpl in H. 
+      apply notin_singleton_1' in H. 
+      destruct (x0 == x). contradiction. reflexivity.
+    - rewrite IHt1. rewrite IHt2. reflexivity.
+      simpl in H. 
+      + apply notin_union_2 in H. apply H.
+      + apply notin_union_1 in H. apply H.
+    - f_equal. simpl in H. 
+Abort. 
+    
+       
 
      
     
